PivotBetree/BucketsLib.i.dfy
@@ -18,19 +18,31 @@ module BucketsLib {
   import opened KeyType
   import UI
 
-  type Bucket = map<Key, Message>
+  // If a bucket on disk is ill-formed, but in a way
+  // that our basic sanity checks don't detect, then
+  // it will map to a bucket with wellMarshalled=false
+
+  type BucketMap = map<Key, Message>
+  datatype Bucket = Bucket(b: BucketMap) | IllMarshalledBucket
   type BucketList = seq<Bucket>
 
   predicate {:opaque} WFBucket(bucket: Bucket)
   {
-    && (forall key | key in bucket :: bucket[key] != IdentityMessage())
+    bucket.Bucket? ==> (forall key | key in bucket.b :: bucket.b[key] != IdentityMessage())
+  }
+
+  predicate BucketListWellMarshalled(blist: BucketList)
+  {
+    forall i | 0 <= i < |blist| :: blist[i].Bucket?
   }
 
   predicate WFBucketAt(bucket: Bucket, pivots: PivotTable, i: int)
   requires WFPivots(pivots)
   {
-    && (forall key | key in bucket :: bucket[key] != IdentityMessage())
-    && (forall key | key in bucket :: Route(pivots, key) == i)
+    bucket.Bucket? ==> (
+      && (forall key | key in bucket.b :: bucket.b[key] != IdentityMessage())
+      && (forall key | key in bucket.b :: Route(pivots, key) == i)
+    )
   }
 
   predicate WFBucketList(blist: BucketList, pivots: PivotTable)
@@ -41,27 +53,31 @@ module BucketsLib {
   }
 
   function BucketGet(bucket: Bucket, key: Key) : Message
+  requires bucket.Bucket?
   {
-    if key in bucket then bucket[key] else IdentityMessage()
+    if key in bucket.b then bucket.b[key] else IdentityMessage()
   }
 
   function BucketListGet(blist: BucketList, pivots: PivotTable, key: Key) : Message
   requires WFBucketList(blist, pivots)
+  requires BucketListWellMarshalled(blist);
   {
     BucketGet(blist[Route(pivots, key)], key)
   }
 
   function BucketInsert(bucket: Bucket, key: Key, msg: Message) : Bucket
+  requires bucket.Bucket?
   {
     var mergedMsg := Merge(msg, BucketGet(bucket, key));
     if mergedMsg == IdentityMessage() then
-      MapRemove1(bucket, key)
+      Bucket(MapRemove1(bucket.b, key))
     else
-      bucket[key := mergedMsg]
+      Bucket(bucket.b[key := mergedMsg])
   }
 
   function BucketListInsert(blist: BucketList, pivots: PivotTable, key: Key, msg: Message) : BucketList
   requires WFBucketList(blist, pivots)
+  requires blist[Route(pivots, key)].Bucket?
   {
     var i := Route(pivots, key);
     blist[i := BucketInsert(blist[i], key, msg)]
@@ -71,17 +87,22 @@ module BucketsLib {
   // messages from the parent destined for this child.
   function BucketListItemFlush(parent: Bucket, child: Bucket, pivots: PivotTable, i: int) : Bucket
   requires WFPivots(pivots)
+  requires parent.Bucket?
+  requires child.Bucket?
   {
-    map key
-    | && (key in (child.Keys + parent.Keys)) // this is technically redundant but allows Dafny to figure out that the domain is finite
+    Bucket(map key
+    | && (key in (child.b.Keys + parent.b.Keys)) // this is technically redundant but allows Dafny to figure out that the domain is finite
       && Route(pivots, key) == i
       && Merge(BucketGet(parent, key), BucketGet(child, key)) != IdentityMessage()
     :: Merge(BucketGet(parent, key), BucketGet(child, key))
+    )
   }
 
   function BucketListFlushPartial(parent: Bucket, children: BucketList, pivots: PivotTable, i: int) : (res : BucketList)
   requires WFPivots(pivots)
   requires 0 <= i <= |children|
+  requires parent.Bucket?
+  requires BucketListWellMarshalled(children)
   ensures |res| == i
   ensures forall h :: 0 <= h < i ==> res[h] == BucketListItemFlush(parent, children[h], pivots, h);
   {
@@ -92,48 +113,63 @@ module BucketsLib {
 
   function BucketListFlush(parent: Bucket, children: BucketList, pivots: PivotTable) : (res : BucketList)
   requires WFPivots(pivots)
+  requires parent.Bucket?
+  requires BucketListWellMarshalled(children)
   ensures |res| == |children|
+  ensures BucketListWellMarshalled(res)
   ensures forall h :: 0 <= h < |res| ==> res[h] == BucketListItemFlush(parent, children[h], pivots, h);
   {
     BucketListFlushPartial(parent, children, pivots, |children|)
   }
 
   function JoinBucketList(buckets: seq<Bucket>) : (bucket : Bucket)
+  requires BucketListWellMarshalled(buckets)
+  ensures bucket.Bucket?
   {
-    if |buckets| == 0 then map[] else MapUnion(JoinBucketList(DropLast(buckets)), Last(buckets))
+    if |buckets| == 0 then Bucket(map[]) else Bucket(MapUnion(JoinBucketList(DropLast(buckets)).b, Last(buckets).b))
   }
 
   function SplitBucketOnPivots(bucket: Bucket, pivots: seq<Key>) : (buckets: BucketList)
+  requires bucket.Bucket?
   ensures |buckets| == |pivots| + 1
+  ensures BucketListWellMarshalled(buckets)
+  decreases |pivots|
   {
     if |pivots| == 0 then (
       [bucket]
     ) else (
-      var l := map key | key in bucket && Keyspace.lt(key, Last(pivots)) :: bucket[key];
-      var r := map key | key in bucket && Keyspace.lte(Last(pivots), key) :: bucket[key];
+      var l := Bucket(map key | key in bucket.b && Keyspace.lt(key, Last(pivots)) :: bucket.b[key]);
+      var r := Bucket(map key | key in bucket.b && Keyspace.lte(Last(pivots), key) :: bucket.b[key]);
 
       SplitBucketOnPivots(l, DropLast(pivots)) + [r]
     )
   }
 
-  function ClampToSlot(bucket: Bucket, pivots: PivotTable, i: int) : Bucket
+  function ClampToSlot(bucket: Bucket, pivots: PivotTable, i: int) : (res : Bucket)
   requires WFPivots(pivots)
+  requires bucket.Bucket?
+  ensures res.Bucket?
   {
-    map key | key in bucket && Route(pivots, key) == i :: bucket[key]
+    Bucket(map key | key in bucket.b && Route(pivots, key) == i :: bucket.b[key])
   }
 
-  function {:opaque} BucketIntersect(bucket: Bucket, keys: set<Key>) : Bucket
+  function {:opaque} BucketIntersect(bucket: Bucket, keys: set<Key>) : (res : Bucket)
+  requires bucket.Bucket?
+  ensures res.Bucket?
   {
-    map key | key in bucket && key in keys :: bucket[key]
+    Bucket(map key | key in bucket.b && key in keys :: bucket.b[key])
   }
 
-  function {:opaque} BucketComplement(bucket: Bucket, keys: set<Key>) : Bucket
+  function {:opaque} BucketComplement(bucket: Bucket, keys: set<Key>) : (res : Bucket)
+  requires bucket.Bucket?
+  ensures res.Bucket?
   {
-    map key | key in bucket && key !in keys :: bucket[key]
+    Bucket(map key | key in bucket.b && key !in keys :: bucket.b[key])
   }
 
   lemma WFBucketIntersect(bucket: Bucket, keys: set<Key>)
   requires WFBucket(bucket)
+  requires bucket.Bucket?
   ensures WFBucket(BucketIntersect(bucket, keys))
   {
     reveal_WFBucket();
@@ -142,6 +178,7 @@ module BucketsLib {
 
   lemma WFBucketComplement(bucket: Bucket, keys: set<Key>)
   requires WFBucket(bucket)
+  requires bucket.Bucket?
   ensures WFBucket(BucketComplement(bucket, keys))
   {
     reveal_WFBucket();
@@ -152,26 +189,36 @@ module BucketsLib {
 
   // Note: does NOT necessarily return a WFBucket!
   // It might contain NoOp messages
-  function {:opaque} Compose(top: Bucket, bot: Bucket) : Bucket
+  function {:opaque} Compose(top: Bucket, bot: Bucket) : (res : Bucket)
+  requires top.Bucket?
+  requires bot.Bucket?
+  ensures res.Bucket?
   {
-    map key
-    | key in (top.Keys + bot.Keys)
+    Bucket(map key
+    | key in (top.b.Keys + bot.b.Keys)
     :: Merge(BucketGet(top, key), BucketGet(bot, key))
+    )
   }
 
-  function {:opaque} ComposeSeq(buckets: seq<Bucket>) : Bucket
+  function {:opaque} ComposeSeq(buckets: seq<Bucket>) : (res : Bucket)
+  requires BucketListWellMarshalled(buckets)
+  ensures res.Bucket?
   {
-    if |buckets| == 0 then map[] else Compose(ComposeSeq(DropLast(buckets)), Last(buckets))
+    if |buckets| == 0 then Bucket(map[]) else Compose(ComposeSeq(DropLast(buckets)), Last(buckets))
   }
 
   lemma ComposeSeq1(b: Bucket)
-  ensures ComposeSeq([b]) == b
+  requires b.Bucket?
+  ensures ComposeSeq([b]) == Bucket(b.b)
   {
     reveal_Compose();
     reveal_ComposeSeq();
   }
 
   lemma ComposeAssoc(a: Bucket, b: Bucket, c: Bucket)
+  requires a.Bucket?
+  requires b.Bucket?
+  requires c.Bucket?
   ensures Compose(Compose(a, b), c) == Compose(a, Compose(b, c))
   {
     reveal_Compose();
@@ -182,6 +229,9 @@ module BucketsLib {
   }
 
   lemma ComposeSeqAdditive(a: seq<Bucket>, b: seq<Bucket>)
+  requires BucketListWellMarshalled(a)
+  requires BucketListWellMarshalled(b)
+  ensures BucketListWellMarshalled(a + b)
   ensures ComposeSeq(a + b) == Compose(ComposeSeq(a), ComposeSeq(b))
   {
     reveal_ComposeSeq();
@@ -191,7 +241,7 @@ module BucketsLib {
       assert a + b == a;
       assert ComposeSeq(a + b)
           == ComposeSeq(a)
-          == Compose(ComposeSeq(a), map[])
+          == Compose(ComposeSeq(a), Bucket(map[]))
           == Compose(ComposeSeq(a), ComposeSeq(b));
     } else {
       ComposeSeqAdditive(a, b[..|b|-1]);
@@ -208,6 +258,7 @@ module BucketsLib {
   }
 
   function InterpretBucketStack(buckets: seq<Bucket>, key: Key) : Message
+  requires BucketListWellMarshalled(buckets)
   {
     if |buckets| == 0 then
       Update(NopDelta())
@@ -216,6 +267,7 @@ module BucketsLib {
   }
 
   lemma BucketGetComposeSeq(buckets: seq<Bucket>, key: Key)
+  requires BucketListWellMarshalled(buckets)
   ensures BucketGet(ComposeSeq(buckets), key) == InterpretBucketStack(buckets, key);
   {
     reveal_ComposeSeq();
@@ -229,26 +281,30 @@ module BucketsLib {
   ////// Clamping based on RangeStart and RangeEnd
 
   function {:opaque} ClampRange(bucket: Bucket, start: UI.RangeStart, end: UI.RangeEnd) : Bucket
+  requires bucket.Bucket?
   {
-    map key | key in bucket && MS.InRange(start, key, end) :: bucket[key]
+    Bucket(map key | key in bucket.b && MS.InRange(start, key, end) :: bucket.b[key])
   }
 
   function {:opaque} ClampStart(bucket: Bucket, start: UI.RangeStart) : Bucket
+  requires bucket.Bucket?
   {
-    map key | key in bucket && MS.LowerBound(start, key) :: bucket[key]
+    Bucket(map key | key in bucket.b && MS.LowerBound(start, key) :: bucket.b[key])
   }
 
   function {:opaque} ClampEnd(bucket: Bucket, end: UI.RangeEnd) : Bucket
+  requires bucket.Bucket?
   {
-    map key | key in bucket && MS.UpperBound(key, end) :: bucket[key]
+    Bucket(map key | key in bucket.b && MS.UpperBound(key, end) :: bucket.b[key])
   }
 
   ///// KeyValueMapOfBucket
 
   function {:opaque} KeyValueMapOfBucket(bucket: Bucket) : map<Key, Value>
+  requires bucket.Bucket?
   {
-    map key | key in bucket && Merge(bucket[key], DefineDefault()).value != DefaultValue()
-      :: Merge(bucket[key], DefineDefault()).value
+    map key | key in bucket.b && Merge(bucket.b[key], DefineDefault()).value != DefaultValue()
+      :: Merge(bucket.b[key], DefineDefault()).value
   }
 
   function {:opaque} SortedSeqOfKeyValueMap(m: map<Key, Value>) : seq<UI.SuccResult>
@@ -316,19 +372,24 @@ module BucketsLib {
   ///// Splitting stuff
 
   // NB(jonh): These definitions are timeout monsters.
-  function {:opaque} SplitBucketLeft(bucket: Bucket, pivot: Key) : Bucket
+  function {:opaque} SplitBucketLeft(bucket: Bucket, pivot: Key) : (res : Bucket)
+  requires bucket.Bucket?
+  ensures res.Bucket?
   {
-    map key | key in bucket && Keyspace.lt(key, pivot) :: bucket[key]
+    Bucket(map key | key in bucket.b && Keyspace.lt(key, pivot) :: bucket.b[key])
   }
 
-  function {:opaque} SplitBucketRight(bucket: Bucket, pivot: Key) : Bucket
+  function {:opaque} SplitBucketRight(bucket: Bucket, pivot: Key) : (res : Bucket)
+  requires bucket.Bucket?
+  ensures res.Bucket?
   {
-    map key | key in bucket && Keyspace.lte(pivot, key) :: bucket[key]
+    Bucket(map key | key in bucket.b && Keyspace.lte(pivot, key) :: bucket.b[key])
   }
 
   function SplitBucketListLeft(blist: BucketList, pivots: PivotTable, cLeft: int, key: Key) : BucketList
   requires WFBucketList(blist, pivots)
   requires CutoffForLeft(pivots, key) == cLeft
+  requires blist[cLeft].Bucket?
   {
     blist[.. cLeft] + [SplitBucketLeft(blist[cLeft], key)]
   }
@@ -336,12 +397,14 @@ module BucketsLib {
   function SplitBucketListRight(blist: BucketList, pivots: PivotTable, cRight: int, key: Key) : BucketList
   requires WFBucketList(blist, pivots)
   requires CutoffForRight(pivots, key) == cRight
+  requires blist[cRight].Bucket?
   {
     [SplitBucketRight(blist[cRight], key)] + blist[cRight + 1 ..]
   }
 
   function {:opaque} SplitBucketInList(blist: BucketList, slot: int, pivot: Key) : BucketList
   requires 0 <= slot < |blist|
+  requires blist[slot].Bucket?
   {
     replace1with2(blist,
         SplitBucketLeft(blist[slot], pivot),
@@ -349,14 +412,20 @@ module BucketsLib {
         slot)
   }
 
-  function {:opaque} MergeBuckets(left: Bucket, right: Bucket) : Bucket
+  function {:opaque} MergeBuckets(left: Bucket, right: Bucket) : (res : Bucket)
+  requires left.Bucket?
+  requires right.Bucket?
+  ensures res.Bucket?
   {
-    MapUnionPreferA(left, right)
+    Bucket(MapUnionPreferA(left.b, right.b))
   }
 
   function {:opaque} MergeBucketsInList(blist: BucketList, slot: int) : (blist' : BucketList)
   requires 0 <= slot < |blist| - 1
+  requires blist[slot].Bucket?
+  requires blist[slot+1].Bucket?
   ensures |blist'| == |blist| - 1
+  ensures blist'[slot].Bucket?
   {
     replace2with1(blist,
         MergeBuckets(blist[slot], blist[slot+1]),
@@ -367,12 +436,13 @@ module BucketsLib {
   requires 0 <= i <= |pivots|
   requires WFPivots(pivots)
   requires WFBucketAt(bucket, pivots, i)
+  requires bucket.Bucket?
   ensures WFPivots(pivots[.. i])
   ensures WFBucketAt(SplitBucketLeft(bucket, pivot), pivots[.. i], i)
   {
     reveal_SplitBucketLeft();
     WFSlice(pivots, 0, i);
-    forall key | key in SplitBucketLeft(bucket, pivot)
+    forall key | key in SplitBucketLeft(bucket, pivot).b
     ensures Route(pivots[.. i], key) == i
     {
       RouteIs(pivots[.. i], key, i);
@@ -383,12 +453,13 @@ module BucketsLib {
   requires 0 <= i <= |pivots|
   requires WFPivots(pivots)
   requires WFBucketAt(bucket, pivots, i)
+  requires bucket.Bucket?
   ensures WFPivots(pivots[i ..])
   ensures WFBucketAt(SplitBucketRight(bucket, pivot), pivots[i ..], 0)
   {
     reveal_SplitBucketRight();
     WFSuffix(pivots, i);
-    forall key | key in SplitBucketRight(bucket, pivot)
+    forall key | key in SplitBucketRight(bucket, pivot).b
     ensures Route(pivots[i ..], key) == 0
     {
       RouteIs(pivots[i ..], key, 0);
@@ -398,16 +469,17 @@ module BucketsLib {
   lemma WFSplitBucketListLeft(blist: BucketList, pivots: PivotTable, cLeft: int, key: Key)
   requires WFBucketList(blist, pivots)
   requires CutoffForLeft(pivots, key) == cLeft
+  requires blist[cLeft].Bucket?
   ensures WFBucketList(SplitBucketListLeft(blist, pivots, cLeft, key), pivots[.. cLeft])
   {
     reveal_SplitBucketLeft();
     WFSlice(pivots, 0, cLeft);
 
     var res := SplitBucketListLeft(blist, pivots, cLeft, key);
-    forall i | 0 <= i < |res|
+    forall i | 0 <= i < |res| && res[i].Bucket?
     ensures WFBucketAt(res[i], pivots[..cLeft], i)
     {
-      forall key | key in res[i]
+      forall key | key in res[i].b
       ensures Route(pivots[..cLeft], key) == i
       {
         RouteIs(pivots[..cLeft], key, i);
@@ -418,16 +490,17 @@ module BucketsLib {
   lemma WFSplitBucketListRight(blist: BucketList, pivots: PivotTable, cRight: int, key: Key)
   requires WFBucketList(blist, pivots)
   requires CutoffForRight(pivots, key) == cRight
+  requires blist[cRight].Bucket?
   ensures WFBucketList(SplitBucketListRight(blist, pivots, cRight, key), pivots[cRight ..])
   {
     reveal_SplitBucketRight();
     WFSuffix(pivots, cRight);
 
     var res := SplitBucketListRight(blist, pivots, cRight, key);
-    forall i | 0 <= i < |res|
+    forall i | 0 <= i < |res| && res[i].Bucket?
     ensures WFBucketAt(res[i], pivots[cRight..], i)
     {
-      forall key | key in res[i]
+      forall key | key in res[i].b
       ensures Route(pivots[cRight..], key) == i
       {
         RouteIs(pivots[cRight..], key, i);
@@ -438,6 +511,7 @@ module BucketsLib {
   lemma WFSplitBucketInList(blist: BucketList, slot: int, pivot: Key, pivots: PivotTable)
   requires WFBucketList(blist, pivots)
   requires 0 <= slot < |blist|
+  requires blist[slot].Bucket?
   requires PivotInsertable(pivots, slot, pivot)
   ensures WFPivots(insert(pivots, pivot, slot))
   ensures WFBucketList(SplitBucketInList(blist, slot, pivot), insert(pivots, pivot, slot))
@@ -473,19 +547,19 @@ module BucketsLib {
   requires forall i | a <= i < b :: pivots'[i] == pivots[i-d]
   requires b >= a && b < |pivots'| ==> (
       || (b-d < |pivots| && pivots'[b] == pivots[b-d])
-      || (forall key | key in blist'[b] :: Keyspace.lt(key, pivots'[b]))
+      || (blist'[b].Bucket? ==> forall key | key in blist'[b].b :: Keyspace.lt(key, pivots'[b]))
     )
   requires b >= a && a-1 >= 0 ==> (
       || (a-1-d >= 0 && pivots'[a-1] == pivots[a-1-d])
-      || (forall key | key in blist'[a] :: Keyspace.lte(pivots'[a-1], key))
+      || (blist'[a].Bucket? ==> forall key | key in blist'[a].b :: Keyspace.lte(pivots'[a-1], key))
     )
   ensures forall i | a <= i <= b :: WFBucketAt(blist'[i], pivots', i)
   {
-    forall i | a <= i <= b
+    forall i | a <= i <= b && blist'[i].Bucket?
     ensures WFBucketAt(blist'[i], pivots', i)
     {
       assert WFBucketAt(blist[i-d], pivots, i - d);
-      forall key | key in blist'[i]
+      forall key | key in blist'[i].b
       {
         RouteIs(pivots', key, i);
       }
@@ -495,6 +569,8 @@ module BucketsLib {
   lemma WFMergeBucketsInList(blist: BucketList, slot: int, pivots: PivotTable)
   requires 0 <= slot < |blist| - 1
   requires WFBucketList(blist, pivots)
+  requires blist[slot].Bucket?
+  requires blist[slot+1].Bucket?
   ensures WFBucketList(MergeBucketsInList(blist, slot), remove(pivots, slot))
   {
     reveal_MergeBucketsInList();
@@ -512,6 +588,8 @@ module BucketsLib {
   lemma SplitOfMergeBucketsInList(blist: BucketList, slot: int, pivots: PivotTable)
   requires 0 <= slot < |blist| - 1
   requires WFBucketList(blist, pivots)
+  requires blist[slot].Bucket?
+  requires blist[slot+1].Bucket?
   ensures SplitBucketLeft(MergeBucketsInList(blist, slot)[slot], pivots[slot]) == blist[slot]
   ensures SplitBucketRight(MergeBucketsInList(blist, slot)[slot], pivots[slot]) == blist[slot+1]
   {
@@ -525,6 +603,7 @@ module BucketsLib {
 
   lemma WFJoinBucketList(buckets: seq<Bucket>)
   requires forall i | 0 <= i < |buckets| :: WFBucket(buckets[i])
+  requires BucketListWellMarshalled(buckets)
   ensures WFBucket(JoinBucketList(buckets))
   {
     reveal_WFBucket();
@@ -537,6 +616,8 @@ module BucketsLib {
   lemma BucketListFlushPartialAt(parent: Bucket, blist: BucketList, pivots: PivotTable, j: int, i: int)
   requires 0 <= i < j <= |blist|
   requires WFPivots(pivots)
+  requires parent.Bucket?
+  requires BucketListWellMarshalled(blist)
   ensures BucketListFlushPartial(parent, blist, pivots, j)[i] == BucketListItemFlush(parent, blist[i], pivots, i)
   {
     if j == i + 1 {
@@ -548,6 +629,8 @@ module BucketsLib {
   lemma BucketListFlushAt(parent: Bucket, blist: BucketList, pivots: PivotTable, i: int)
   requires 0 <= i < |blist|
   requires WFPivots(pivots)
+  requires parent.Bucket?
+  requires BucketListWellMarshalled(blist)
   ensures BucketListFlush(parent, blist, pivots)[i] == BucketListItemFlush(parent, blist[i], pivots, i)
   {
     BucketListFlushPartialAt(parent, blist, pivots, |blist|, i);
@@ -555,6 +638,8 @@ module BucketsLib {
 
   lemma WFBucketListFlush(parent: Bucket, blist: BucketList, pivots: PivotTable)
   requires WFBucketList(blist, pivots)
+  requires parent.Bucket?
+  requires BucketListWellMarshalled(blist)
   ensures WFBucketList(BucketListFlush(parent, blist, pivots), pivots)
   {
     var f := BucketListFlush(parent, blist, pivots);
@@ -567,6 +652,8 @@ module BucketsLib {
 
   lemma GetBucketListFlushEqMerge(parent: Bucket, blist: BucketList, pivots: PivotTable, key: Key)
   requires WFBucketList(blist, pivots)
+  requires parent.Bucket?
+  requires BucketListWellMarshalled(blist)
   ensures WFBucketList(BucketListFlush(parent, blist, pivots), pivots)
   ensures BucketListGet(BucketListFlush(parent, blist, pivots), pivots, key)
       == Merge(BucketGet(parent, key), BucketListGet(blist, pivots, key))
@@ -578,12 +665,13 @@ module BucketsLib {
 
   lemma KeyInJoinedBucketsInSomeBucket(buckets: seq<Bucket>, key: Key)
   returns (i : int)
-  requires key in JoinBucketList(buckets)
+  requires BucketListWellMarshalled(buckets)
+  requires key in JoinBucketList(buckets).b
   ensures 0 <= i < |buckets|
-  ensures key in buckets[i]
+  ensures key in buckets[i].b
   {
     assert |buckets| > 0;
-    if key in Last(buckets) {
+    if key in Last(buckets).b {
       i := |buckets| - 1;
     } else {
       i := KeyInJoinedBucketsInSomeBucket(DropLast(buckets), key);
@@ -591,6 +679,7 @@ module BucketsLib {
   }
 
   lemma GetJoinBucketListEq(blist: BucketList, pivots: PivotTable, key: Key)
+  requires BucketListWellMarshalled(blist)
   requires WFBucketList(blist, pivots)
   ensures BucketGet(JoinBucketList(blist), key) == BucketListGet(blist, pivots, key)
   {
@@ -607,7 +696,7 @@ module BucketsLib {
       {
         var bucket := DropLast(blist)[i];
         assert WFBucketAt(blist[i], pivots, i);
-        forall key | key in bucket ensures Route(DropLast(pivots), key) == i {
+        forall key | key in bucket.b ensures Route(DropLast(pivots), key) == i {
           RouteIs(DropLast(pivots), key, i);
         }
       }
@@ -620,14 +709,14 @@ module BucketsLib {
         //  assert Keyspace.lte(piv, key);
         //  assert false;
         //}
-        assert key !in b2;
+        assert key !in b2.b;
         assert BucketGet(blist[Route(pivots, key)], key) == BucketGet(JoinBucketList(blist), key);
       } else {
-        if (key in b1) {
+        if (key in b1.b) {
           var i := KeyInJoinedBucketsInSomeBucket(DropLast(blist), key);
           assert false;
         }
-        assert key !in b1;
+        assert key !in b1.b;
         assert BucketGet(blist[Route(pivots, key)], key) == BucketGet(JoinBucketList(blist), key);
       }
     }
@@ -635,75 +724,96 @@ module BucketsLib {
 
   lemma BucketListItemFlushAddParentKey(parent: Bucket, child: Bucket, pivots: PivotTable, key: Key, msg: Message)
   requires WFPivots(pivots)
-  requires key !in parent
-  requires key !in child
+  requires parent.Bucket?
+  requires child.Bucket?
+  requires key !in parent.b
+  requires key !in child.b
   requires msg != IdentityMessage()
-  ensures BucketListItemFlush(parent, child, pivots, Route(pivots, key))[key := msg]
-      == BucketListItemFlush(parent[key := msg], child, pivots, Route(pivots, key))
+  ensures Bucket(BucketListItemFlush(parent, child, pivots, Route(pivots, key)).b[key := msg])
+      == BucketListItemFlush(Bucket(parent.b[key := msg]), child, pivots, Route(pivots, key))
   {
+    assert BucketListItemFlush(parent, child, pivots, Route(pivots, key)).b[key := msg]
+        == BucketListItemFlush(Bucket(parent.b[key := msg]), child, pivots, Route(pivots, key)).b;
   }
 
   lemma BucketListItemFlushAddChildKey(parent: Bucket, child: Bucket, pivots: PivotTable, key: Key, msg: Message)
   requires WFPivots(pivots)
-  requires key !in parent
-  requires key !in child
+  requires parent.Bucket?
+  requires child.Bucket?
+  requires key !in parent.b
+  requires key !in child.b
   requires msg != IdentityMessage()
-  ensures BucketListItemFlush(parent, child, pivots, Route(pivots, key))[key := msg]
-      == BucketListItemFlush(parent, child[key := msg], pivots, Route(pivots, key))
+  ensures Bucket(BucketListItemFlush(parent, child, pivots, Route(pivots, key)).b[key := msg])
+      == BucketListItemFlush(parent, Bucket(child.b[key := msg]), pivots, Route(pivots, key))
   {
+    assert BucketListItemFlush(parent, child, pivots, Route(pivots, key)).b[key := msg]
+        == BucketListItemFlush(parent, Bucket(child.b[key := msg]), pivots, Route(pivots, key)).b;
   }
 
   lemma BucketListItemFlushAddParentAndChildKey(parent: Bucket, child: Bucket, pivots: PivotTable, key: Key, msgParent: Message, msgChild: Message)
   requires WFPivots(pivots)
-  requires key !in parent
-  requires key !in child
+  requires parent.Bucket?
+  requires child.Bucket?
+  requires key !in parent.b
+  requires key !in child.b
   requires ValueMessage.Merge(msgParent, msgChild) != IdentityMessage()
-  ensures BucketListItemFlush(parent, child, pivots, Route(pivots, key))[key := ValueMessage.Merge(msgParent, msgChild)]
-      == BucketListItemFlush(parent[key := msgParent], child[key := msgChild], pivots, Route(pivots, key))
+  ensures Bucket(BucketListItemFlush(parent, child, pivots, Route(pivots, key)).b[key := ValueMessage.Merge(msgParent, msgChild)])
+      == BucketListItemFlush(Bucket(parent.b[key := msgParent]), Bucket(child.b[key := msgChild]), pivots, Route(pivots, key))
   {
+    assert BucketListItemFlush(parent, child, pivots, Route(pivots, key)).b[key := ValueMessage.Merge(msgParent, msgChild)]
+        == BucketListItemFlush(Bucket(parent.b[key := msgParent]), Bucket(child.b[key := msgChild]), pivots, Route(pivots, key)).b;
   }
 
   lemma BucketListItemFlushEmpty(pivots: seq<Key>)
   requires WFPivots(pivots)
-  ensures BucketListItemFlush(map[], map[], pivots, 0) == map[]
+  ensures BucketListItemFlush(Bucket(map[]), Bucket(map[]), pivots, 0) == Bucket(map[])
   {
+    assert BucketListItemFlush(Bucket(map[]), Bucket(map[]), pivots, 0).b == map[];
   }
 
-  lemma BucketListItemFlushOfKeysLt(m: map<Key, Message>, pivots: seq<Key>, i: int)
+  lemma BucketListItemFlushOfKeysLt(m: Bucket, pivots: seq<Key>, i: int)
   requires WFPivots(pivots)
+  requires m.Bucket?
   requires 0 <= i < |pivots|
-  requires forall key | key in m :: lt(key, pivots[i])
-  ensures BucketListItemFlush(m, map[], pivots, i+1) == map[]
+  requires forall key | key in m.b :: lt(key, pivots[i])
+  ensures BucketListItemFlush(m, Bucket(map[]), pivots, i+1) == Bucket(map[])
   {
   }
 
   lemma BucketListItemFlushEq(p1: Bucket, p2: Bucket, child: Bucket, pivots: seq<Key>, i: int)
   requires WFPivots(pivots)
+  requires p1.Bucket?
+  requires p2.Bucket?
+  requires child.Bucket?
   requires 0 <= i <= |pivots|
-  requires forall key | Route(pivots, key) == i :: MapsAgreeOnKey(p1, p2, key)
+  requires forall key | Route(pivots, key) == i :: MapsAgreeOnKey(p1.b, p2.b, key)
   ensures BucketListItemFlush(p1, child, pivots, i)
        == BucketListItemFlush(p2, child, pivots, i)
   {
+    assert BucketListItemFlush(p1, child, pivots, i).b
+        == BucketListItemFlush(p2, child, pivots, i).b;
   }
 
-  lemma SplitBucketOnPivotsAt(bucket: map<Key, Message>, pivots: seq<Key>, i: int)
+  lemma SplitBucketOnPivotsAt(bucket: Bucket, pivots: seq<Key>, i: int)
   requires WFPivots(pivots)
+  requires bucket.Bucket?
   requires 0 <= i <= |pivots|
   ensures SplitBucketOnPivots(bucket, pivots)[i] == ClampToSlot(bucket, pivots, i)
+  decreases |pivots|
   {
     if i == |pivots| {
     } else {
-      var l := map key | key in bucket && lt(key, Last(pivots)) :: bucket[key];
+      var l := map key | key in bucket.b && lt(key, Last(pivots)) :: bucket.b[key];
       WFSlice(pivots, 0, |pivots| - 1);
-      SplitBucketOnPivotsAt(l, DropLast(pivots), i);
-      var a := SplitBucketOnPivots(bucket, pivots)[i];
-      var b := map key | key in bucket && Route(pivots, key) == i :: bucket[key];
+      SplitBucketOnPivotsAt(Bucket(l), DropLast(pivots), i);
+      var a := SplitBucketOnPivots(bucket, pivots)[i].b;
+      var b := map key | key in bucket.b && Route(pivots, key) == i :: bucket.b[key];
 
       forall key | key in a
       ensures key in b
       ensures a[key] == b[key];
       {
-        assert key in bucket;
+        assert key in bucket.b;
         RouteIs(pivots, key, i);
       }
 
@@ -720,16 +830,18 @@ module BucketsLib {
     }
   }
 
-  lemma AddMessagesToBucketsEmpAt(bucket: map<Key, Message>, pivots: seq<Key>, emp: seq<map<Key, Message>>, i: int)
+  lemma AddMessagesToBucketsEmpAt(bucket: Bucket, pivots: seq<Key>, emp: BucketList, i: int)
   requires WFPivots(pivots)
+  requires bucket.Bucket?
   requires 0 <= i <= |pivots|
   requires |emp| == |pivots| + 1
-  requires forall i | 0 <= i < |emp| :: emp[i] == map[]
-  requires forall key | key in bucket :: bucket[key] != IdentityMessage();
-  ensures BucketListFlush(bucket, emp, pivots)[i] == map key | key in bucket && Route(pivots, key) == i :: bucket[key]
+  requires forall i | 0 <= i < |emp| :: emp[i] == Bucket(map[])
+  requires forall key | key in bucket.b :: bucket.b[key] != IdentityMessage();
+  ensures BucketListFlush(bucket, emp, pivots)[i]
+       == Bucket(map key | key in bucket.b && Route(pivots, key) == i :: bucket.b[key])
   {
-    var a := BucketListFlush(bucket, emp, pivots)[i];
-    var b := map key | key in bucket && Route(pivots, key) == i :: bucket[key];
+    var a := BucketListFlush(bucket, emp, pivots)[i].b;
+    var b := map key | key in bucket.b && Route(pivots, key) == i :: bucket.b[key];
     forall key | key in a
     ensures key in b
     ensures a[key] == b[key];
@@ -751,11 +863,12 @@ module BucketsLib {
     assert a == b;
   }
 
-  lemma LemmaSplitBucketOnPivotsEqAddMessagesToBuckets(bucket: map<Key, Message>, pivots: seq<Key>, emp: seq<map<Key, Message>>)
+  lemma LemmaSplitBucketOnPivotsEqAddMessagesToBuckets(bucket: Bucket, pivots: seq<Key>, emp: seq<Bucket>)
   requires WFPivots(pivots)
+  requires bucket.Bucket?
   requires |emp| == |pivots| + 1
-  requires forall i | 0 <= i < |emp| :: emp[i] == map[]
-  requires forall key | key in bucket :: bucket[key] != IdentityMessage();
+  requires forall i | 0 <= i < |emp| :: emp[i] == Bucket(map[])
+  requires forall key | key in bucket.b :: bucket.b[key] != IdentityMessage();
   ensures SplitBucketOnPivots(bucket, pivots) == BucketListFlush(bucket, emp, pivots)
   {
     var a := SplitBucketOnPivots(bucket, pivots);
@@ -773,28 +886,30 @@ module BucketsLib {
   lemma BucketListFlushParentEmpty(blist: BucketList, pivots: PivotTable)
   requires WFPivots(pivots)
   requires WFBucketList(blist, pivots)
-  ensures BucketListFlush(map[], blist, pivots) == blist
+  requires BucketListWellMarshalled(blist);
+  ensures BucketListFlush(Bucket(map[]), blist, pivots) == blist
   {
-    var a := BucketListFlush(map[], blist, pivots);
+    var a := BucketListFlush(Bucket(map[]), blist, pivots);
     var b := blist;
     forall i | 0 <= i < |a|
     ensures a[i] == b[i]
     {
-      BucketListFlushAt(map[], blist, pivots, i);
+      BucketListFlushAt(Bucket(map[]), blist, pivots, i);
     }
   }
 
   function emptyList(n: int) : (l : BucketList)
   requires n >= 0
   ensures |l| == n
-  ensures forall i | 0 <= i < |l| :: l[i] == map[]
+  ensures forall i | 0 <= i < |l| :: l[i] == Bucket(map[])
   {
-    if n == 0 then [] else emptyList(n-1) + [map[]]
+    if n == 0 then [] else emptyList(n-1) + [Bucket(map[])]
   }
 
   lemma WFSplitBucketOnPivots(bucket: Bucket, pivots: seq<Key>)
   requires WFBucket(bucket)
   requires WFPivots(pivots)
+  requires bucket.Bucket?
   ensures WFBucketList(SplitBucketOnPivots(bucket, pivots), pivots)
   {
     reveal_WFBucket();
@@ -806,8 +921,10 @@ module BucketsLib {
   lemma JoinBucketsSplitBucketOnPivotsCancel(bucket: Bucket, pivots: seq<Key>)
   requires WFPivots(pivots)
   requires WFBucket(bucket)
+  requires bucket.Bucket?
   ensures WFBucketList(SplitBucketOnPivots(bucket, pivots), pivots)
   ensures JoinBucketList(SplitBucketOnPivots(bucket, pivots)) == bucket
+  decreases |pivots|
   {
     WFSplitBucketOnPivots(bucket, pivots);
     reveal_WFBucket();
@@ -815,30 +932,30 @@ module BucketsLib {
     if |pivots| == 0 {
     } else {
       var buckets := SplitBucketOnPivots(bucket, pivots);
-      var l := map key | key in bucket && Keyspace.lt(key, Last(pivots)) :: bucket[key];
-      var r := map key | key in bucket && Keyspace.lte(Last(pivots), key) :: bucket[key];
+      var l := map key | key in bucket.b && Keyspace.lt(key, Last(pivots)) :: bucket.b[key];
+      var r := map key | key in bucket.b && Keyspace.lte(Last(pivots), key) :: bucket.b[key];
 
-      var bucketsPref := SplitBucketOnPivots(l, DropLast(pivots));
+      var bucketsPref := SplitBucketOnPivots(Bucket(l), DropLast(pivots));
       WFSlice(pivots, 0, |pivots| - 1);
-      JoinBucketsSplitBucketOnPivotsCancel(l, DropLast(pivots));
+      JoinBucketsSplitBucketOnPivotsCancel(Bucket(l), DropLast(pivots));
 
       forall i | 0 <= i < |buckets|
       ensures WFBucketAt(buckets[i], pivots, i)
       {
         if i < |buckets| - 1 {
           assert WFBucketAt(bucketsPref[i], DropLast(pivots), i);
-          forall key | key in buckets[i] ensures Route(pivots, key) == i
+          forall key | key in buckets[i].b ensures Route(pivots, key) == i
           {
             assert Route(DropLast(pivots), key) == i;
             assert buckets[i] == bucketsPref[i];
-            assert key in bucketsPref[i];
-            SplitBucketOnPivotsAt(l, DropLast(pivots), i);
+            assert key in bucketsPref[i].b;
+            SplitBucketOnPivotsAt(Bucket(l), DropLast(pivots), i);
             assert key in l;
             RouteIs(pivots, key, i);
           }
           assert WFBucketAt(buckets[i], pivots, i);
         } else {
-          forall key | key in buckets[i] ensures Route(pivots, key) == i
+          forall key | key in buckets[i].b ensures Route(pivots, key) == i
           {
             RouteIs(pivots, key, i);
           }
@@ -879,6 +996,8 @@ module BucketsLib {
 
   lemma BucketListInsertBucketListFlush(parent: Bucket, children: BucketList, pivots: PivotTable, key: Key, msg: Message)
   requires WFBucketList(children, pivots)
+  requires parent.Bucket?
+  requires BucketListWellMarshalled(children)
   ensures WFBucketList(BucketListFlush(parent, children, pivots), pivots)
   ensures BucketListInsert(BucketListFlush(parent, children, pivots), pivots, key, msg)
       == BucketListFlush(BucketInsert(parent, key, msg), children, pivots)
